\subsection{Math}
\subsubsection*{Derivative Rules}
Chain rule: $\frac{d}{dx} f(u) = \frac{d}{du} f(u) \cdot \frac{d}{dx} u(x)$\\
Sum/difference rule: $(f \pm g)' = f' \pm g'$\\
Product rule: $(f \cdot g)' = f' \cdot g + f \cdot g'$\\
Quotient rule: $(\frac{f}{g})' = \frac{f' \cdot g - g' \cdot f}{g^2}$\\
\subsubsection*{Common Derivatives}
\fbox{$\frac{d}{dx} a^x = a^x \ln(a)$} \fbox{$\frac{d}{dx} e^x = e^x$}
\fbox{$\frac{d}{dx} \log_a(x) = \frac{1}{x \ln(a)}$} \fbox{$\frac{d}{dx} \ln(x) = \frac{1}{x}$}
\fbox{$\frac{d}{dz} \sigma(z) = \frac{d}{dz} (1 + e^{-z})^{-1} = \sigma(z) (1-\sigma(z))$}
\fbox{$\frac{d}{dx} \tanh(x) = \frac{d}{dx} \frac{e^x - e^{-x}}{e^x + e^{-x}} = 1-\tanh^2(x)$}